cleaning up proofs

coq/Semantics.v
@@ -25,95 +25,6 @@ Fixpoint compile_type (ty : Ty) : Set :=
   | SProduct lhs rhs => compile_type lhs * compile_type rhs
   end.
 
-Program Definition VarEnv_remove (Γ : VarEnv.t) (v : Γ) : VarEnv.t :=
-  VarEnv.make (Subtract _ (VarEnv.vars Γ) (proj1_sig v))
-              (fun v' => VarEnv.lookup Γ v').
-Obligation 1.
-destruct H.
-exact H.
-Defined.
-
-Program Definition weaken_var {Γ : VarEnv.t} {v : Γ} (v' : VarEnv_remove Γ v) : Γ :=
-   v'.
-Obligation 1.
-apply (VarEnv_remove_obligation_1 Γ v).
-Defined.
-
-Lemma shrink_env : forall {Γ ty gs} v,
-  HasTy_VarEnv (((proj1_sig v), ty) :: gs) Γ ->
-  HasTy_VarEnv gs (VarEnv_remove Γ v).
-Proof.
-  intros.
-  eapply HasTy_VarEnv_intro; inversion H.
-  - inversion H0; eauto.
-  - intros.
-    split; intros;
-      specialize (H1 n);
-      inversion H1; clear H1.
-    + clear H5.
-      inversion H3.
-      specialize (H4 H1).
-      inversion H4.
-      exists x.
-      inversion H6.
-      * inversion H7.
-        subst.
-        clear H7.
-        unfold not in H5.
-        exfalso.
-        apply H5.
-        apply In_singleton.
-      * exact H7.
-    + clear H4.
-      unfold VarEnv_remove; simpl.
-      unfold Subtract, Setminus, In in *.
-      split.
-      * inversion H3.
-        eauto using List.in_cons.
-      * unfold not.
-        intros.
-        inversion H1.
-        destruct v.
-        simpl in *.
-        subst.
-        clear H2 H5 H1.
-        inversion H3.
-        clear H3.
-        inversion H0.
-        subst.
-        apply (in_map fst) in H1.
-        simpl in *.
-        contradiction.
-  - intros.
-    split; intros;
-      specialize (H2 (weaken_var v0) ty0);
-      destruct v0 as [n0 Hn0];
-      inversion H2; clear H2.
-    + clear H5.
-      assert (VarEnv.lookup Γ (weaken_var (exist n0 Hn0))
-              = VarEnv.lookup (VarEnv_remove Γ v) (exist n0 Hn0))
-        by (unfold VarEnv_remove, weaken_var; auto);
-      subst.
-      specialize (H4 H2).
-      inversion H4.
-      * inversion H3.
-        destruct v, Hn0.
-        subst; simpl in *.
-        unfold not in n.
-        contradiction n.
-        apply In_singleton.
-      * assumption.
-    + clear H4.
-      apply H5.
-      apply in_cons.
-      unfold weaken_var.
-      unfold weaken_var_obligation_1.
-      unfold VarEnv_remove_obligation_1.
-      destruct Hn0.
-      simpl in *.
-      assumption.
-Qed.
-
 Program Fixpoint LM_state'
          (gs : list GlobalDecl)
          (Γ : VarEnv.t)
@@ -122,17 +33,14 @@ Program Fixpoint LM_state'
   | List.nil => unit
   | (n,ty)::gs' => compile_type ty
                    * LM_state' gs'
-                               (VarEnv_remove Γ n)
-                               (shrink_env n Hty)
+                               (VarEnv.remove Γ n)
+                               (VarEnv_shrink n Hty)
   end.
 Obligation 1.
-inversion Hty.
-specialize (H0 n).
-inversion H0; clear H0.
-clear H2.
-apply H3; clear H3.
-exists ty.
-apply in_eq.
+inversion Hty as [_ Hdom _].
+specialize (Hdom n).
+inversion Hdom.
+eauto using in_eq.
 Qed.
 
 (* Program Definition LM_state (lm : LocalMonitor) (Hty : HasTy_LM lm) : Type := *)
